thys/First_Order_Clause/Ground_Typing.thy
@@ -20,24 +20,32 @@ abbreviation welltyped where "welltyped \<equiv> Ground_Typing.welltyped \<F>"
 
 sublocale explicit_typing where typed = typed and welltyped = welltyped
 proof unfold_locales
+
   show "right_unique typed"
   proof (rule right_uniqueI)
     fix t \<tau>\<^sub>1 \<tau>\<^sub>2
+
     assume "typed t \<tau>\<^sub>1" and "typed t \<tau>\<^sub>2"
+
     thus "\<tau>\<^sub>1 = \<tau>\<^sub>2"
       by (auto elim!: typed.cases)
   qed
 next
-  show welltyped_right_unique: "right_unique welltyped"
+
+  show "right_unique welltyped"
   proof (rule right_uniqueI)
     fix t \<tau>\<^sub>1 \<tau>\<^sub>2
+
     assume "welltyped t \<tau>\<^sub>1" and "welltyped t \<tau>\<^sub>2"
+
     thus "\<tau>\<^sub>1 = \<tau>\<^sub>2"
       by (auto elim!: welltyped.cases)
   qed
 next
   fix t \<tau>
+
   assume "welltyped t \<tau>"
+
   then show "typed t \<tau>"
     by (metis typed.intros welltyped.cases)
 qed
@@ -45,6 +53,7 @@ qed
 sublocale term_typing where typed = typed and welltyped = welltyped and Fun = GFun
 proof unfold_locales
   fix t t' c \<tau> \<tau>'
+
   assume 
     t_type: "welltyped t \<tau>'" and 
     t'_type: "welltyped t' \<tau>'" and
@@ -53,6 +62,7 @@ proof unfold_locales
   from c_type show "welltyped c\<langle>t'\<rangle>\<^sub>G \<tau>"
   proof (induction c arbitrary: \<tau>)
     case Hole
+
     then show ?case
       using t_type t'_type
       by auto
@@ -84,25 +94,33 @@ proof unfold_locales
   qed
 next
   fix t t' c \<tau> \<tau>'
+
   assume "typed t \<tau>'" "typed t' \<tau>'" "typed c\<langle>t\<rangle>\<^sub>G \<tau>"
  
   then show "typed c\<langle>t'\<rangle>\<^sub>G \<tau>"
     by(induction c arbitrary: \<tau>) (auto simp: typed.simps)
 next
   fix f ts \<tau>
+
   assume "welltyped (GFun f ts) \<tau>"
+
   then show "\<forall>t\<in>set ts. is_welltyped t"
     by (metis gterm.inject in_set_conv_nth list_all2_conv_all_nth welltyped.simps)
 next
   fix t
+
   show "is_typed t"
     by (cases t) (meson surj_pair typed.intros)
 qed
 
 end
 
-locale ground_typing = 
-  "term": ground_term_typing + 
-  clause_typing where term_typed = term.typed and term_welltyped = term.welltyped
+locale ground_typing = "term": ground_term_typing
+begin
+
+sublocale clause_typing where term_typed = term.typed and term_welltyped = term.welltyped
+  by unfold_locales
+
+end
 
 end
